\section{Postulates on pure states}

\exo[Evolutions]~

Let $\ket \psi = \ket{0} \otimes \ket{0}$ the initial state of two
qubits. We want to compute $\textit{CNot} (H \otimes I) \ket{\psi}$.

\begin{align*}
  \CNot (H \otimes I) (\ket 0 \otimes \ket 0) &=
    \CNot ((\ket 0 + \ket 1)/\sqrt 2 \otimes (\ket 0 + \ket 1)/\sqrt 2) \\
    &= \frac 1 2 \CNot (\ket{00} + \ket{01} + \ket{10} + \ket{11}) \\
    &= \frac 1 2 (\ket{00} + \ket{01} + \ket{11} + \ket{10}) := \ket{\psi'}
\end{align*}

\begin{align*}
  (H\otimes I)\CNot \ket{\psi'}
  &= (H\otimes I) \frac 1 2 (\ket{00} + \ket{01} + \ket{10} + \ket{11}) \\
  &= \ket {00} & H^2\ket \psi = \ket \psi
\end{align*}

We have $I := H^2$

\begin{enumerate}
  \item $T^4H\; \ket 0$
  \item $HT^4H\; \ket 0$
  \item $\CNot(H \otimes HT^4H)(\ket 0 \otimes \ket 0)$
  \item $(I \otimes \CNot)(\CNot \otimes I)(H \otimes I \otimes I)
    (\ket 0 \otimes \ket 0 \otimes \ket 0)$
  \item $(H \otimes I) (\ket 0 \otimes \ket 0))$
\end{enumerate}

\exo[Measuring in another basis]~

\begin{itemize}
  \item orthogonal :
    \begin{align*}
      \braket + - &= (\frac 1 {\sqrt 2})^2 + \frac 1 {\sqrt 2} \times
          \frac{-1}{\sqrt 2} \\
            &= (\frac 1 {\sqrt 2})^2 - (\frac 1 {\sqrt 2})^2 \\
            &= 0
    \end{align*}

  \item norm one :
    \begin{multicols}{2}
      \begin{align*}
        \braket + + &= (\frac 1 {\sqrt 2})^2 + (\frac 1 {\sqrt 2})^2 \\
            &= \frac 1 2 + \frac 1 2 \\
            &= 1
      \end{align*}

      \begin{align*}
        \braket - - &= (\frac 1 {\sqrt 2})^2 + (\frac{-1}{\sqrt 2})^2 \\
            &= \frac 1 2 + \frac 1 2 \\
            &= 1
      \end{align*}
    \end{multicols}

  \item generate $\mathbb C^2$ 

    Let $c = \alpha \ket 0 + \beta \ket 1 \in \mathbb C^2$ we want to find $x$
    and $y$ such that $x \ket + + y \ket - = c$.

    \begin{align*}
      x \ket + + y \ket - &= 
      \frac x {\sqrt 2}(\ket 0 + \ket 1) + \frac y {\sqrt 2}(\ket 0 - \ket 1) \\
      &= (\frac {x + y} {\sqrt 2}) \ket 0 + (\frac {x - y}{\sqrt 2}) \ket 1
    \end{align*}

    So we have this system :
    \begin{align*}
      \begin{cases}
          (x + y) / \sqrt 2 &= \alpha \\
          (x - y) / \sqrt 2 &= \beta
        \end{cases}
      \Rightarrow& \begin{cases}
          x + y &= \sqrt 2 \alpha \\
          x - y &= \sqrt 2 \beta
        \end{cases} \\
      \Rightarrow& \begin{cases}
          2x &= \sqrt 2 (\alpha + \beta) \\
          x - y &= \sqrt 2 \beta
        \end{cases} \\
      \Rightarrow& \begin{cases}
          x &= \frac {\sqrt 2} 2 (\alpha + \beta) \\
          -x + y &= -\sqrt 2 \beta
        \end{cases} \\
      \Rightarrow& \begin{cases}
          x &= \frac {\sqrt 2} 2 (\alpha + \beta) \\
          y &= \frac {\sqrt 2} 2 (\alpha - \beta)
        \end{cases}
      \end{align*}
\end{itemize}

$B = \{\ket 0, \ket 1\}$ is another o.n.b of $\mathbb C^2$

We need to show that $\sum_{M\in\mathcal M_{\pm}} M^\dagger M = 1$
\begin{align*}
  \sum_{M\in\mathcal M_{\pm}} 
  &= (\ket + \bra +)^\dagger (\ket + \bra +) + 
     (\ket - \bra -)^\dagger (\ket - \bra -) \\
  &= (\ket + \braket + + \bra +) + (\ket - \braket - - \bra -)\\
  &= \ket + \bra + + \ket - \bra - \\
  &= \frac 1 2 (\ket 0 \bra 0 + \ket 0 \bra 1 + \ket 1 \bra 0 + \ket 1 \bra 1) +
     \frac 1 2 (\ket 0 \bra 0 - \ket 0 \bra 1 - \ket 1 \bra 0 + \ket 1 \bra 1)
     \\
  &= \ket 0 \bra 0 + \ket 1 \bra 1 \\
  &= 1
\end{align*}

So $\mathcal M_\pm$ is a valid measurement.

We have $\ket \psi = \frac 1 3 \ket 0 + \frac{\sqrt 8} 3 \ket 1$

\begin{itemize}
  \item For $\ket + \bra +$
    \begin{align*}
      p(\ket +) &= \bra \psi (\ket + \bra +)^\dagger \ket + \bra + \ket \psi \\
      &= \bra \psi \ket + \bra + \ket \psi \\
      &= \braket \psi + \braket + \psi \\
      &= (\frac 1 3 \times \frac 1 {\sqrt 2} + \frac {\sqrt 8} 3 \times \frac 1
        {\sqrt 2})^2 \\
      &= \frac 1 2 \times (\frac{1 + \sqrt 8} 3)^2
      = \frac 1 2 \times \frac {(1 + \sqrt 8)^2} 9
      = \frac {(1 + \sqrt 8)^2}{18}
    \end{align*}

  \item For $\ket - \bra -$
\end{itemize}

\exo[Measuring to distinguish]~

We defined:

\begin{align*}
M_0 = \left(\begin{array}{c c}
  1  & 0\\
  -1 & 0
\end{array}\right)
\quad 
M_+ = \left(\begin{array}{c c}
  1 & -1\\
  2 &  2
\end{array}\right)
\quad
M_f = \left(\begin{array}{c c}
  0 & 0\\
  0 & 0
\end{array}\right)
\end{align*}


