\section{On the nature of quantum information}

\exo[Hadamard]~

\begin{itemize}
  \item $a = 0$
    \begin{align*}
      H \ket 0 &= \frac 1 {\sqrt 2}(\ket 0 + \ket 1)\\
      &= \frac 1 {\sqrt 2}(\ket 0 + (-1)^0 \ket 1)
    \end{align*}
  \item $a = 1$
    \begin{align*}
      H \ket 1 &= \frac 1 {\sqrt 2}(\ket 0 - \ket 1)\\
      &= \frac 1 {\sqrt 2}(\ket 0 + (-1)^1 \ket 1)
    \end{align*}
\end{itemize}

\exo[Who controls whom?]~

We define :
\begin{align*}
\textit{NotC} &=
\left(\begin{array}{c c c c}
  1 & 0 & 0 & 0\\
  0 & 0 & 0 & 1\\
  0 & 0 & 1 & 0\\
  0 & 1 & 0 & 0
\end{array}\right)
\end{align*}
\begin{align*}
\textit{NotC}\ket{00} &= \ket{00}&
\textit{NotC}\ket{01} &= \ket{11} \\
\textit{NotC}\ket{10} &= \ket{10}&
\textit{NotC}\ket{11} &= \ket{01} \\
\end{align*}

We want to proof $(H \otimes H) \CNot (H \otimes H) = \textit{NotC}$ :
\begin{align*}
  (H \otimes H) (\ket x \otimes \ket y) &= (H \ket x \otimes H \ket y) \\
  &= \frac 1 {\sqrt 2}(\ket 0 + (-1)^x \ket 1) \otimes
     \frac 1 {\sqrt 2}(\ket 0 + (-1)^y \ket 1) \\
  &= \frac 1 2 (\ket{00} + (-1)^x \ket{10} + (-1)^y\ket{01} + (-1)^{x+y}\ket{11})
\end{align*}
We apply the operator \CNot :
\begin{align*}
  &\CNot (\frac 1 2 (\ket{00} + (-1)^x \ket{10} + (-1)^y\ket{01} +
  (-1)^{x+y}\ket{11})) \\
  &=\frac 1 2 (\ket{00} + (-1)^x \ket{11} + (-1)^y\ket{01} + (-1)^{x+y}\ket{10})
  \\
  &= \frac 1{\sqrt 2}(\ket 0 + (-1)^{x+y}\ket 1)\otimes (\frac 1{\sqrt 2}(\ket 0 +
  (-1)^y\ket 1)) \\
  &= H\ket{x \oplus y} \otimes H\ket{y} & (-1)^{x+y} = (-1)^{x\oplus y}\; (x
  \oplus y \in \{0, 1\})
\end{align*}
Finlay we apply $(H \otimes H)$:
\begin{align*}
  HH\ket{x\oplus y} \otimes HH\ket y &= \ket{x\oplus y} \otimes \ket y\\
  &= \textit{NotC}(\ket x \otimes \ket y)
\end{align*}


